src/program_proof/rsm/pure/sets.v
@@ -3,7 +3,7 @@ From iris.proofmode Require Import proofmode.
 Section lemmas.
   Context `{SemiSet A C}.
 
-  Lemma set_Forall_subseteq  (P : A -> Prop) (X Y : C) :
+  Lemma set_Forall_subseteq (P : A -> Prop) (X Y : C) :
     X ⊆ Y ->
     set_Forall P Y ->
     set_Forall P X.
